src/Model.Helpers.fst
@@ -3,7 +3,7 @@ module Model.Helpers
 friend Lib.RawIntTypes
 
 let correct #l (b:Seq.seq UInt8.t{Seq.length b = l})
-  : Lemma (reveal #l (hide #l b) == b)
-  [SMTPat (reveal #l (hide #l b))]
+  : Lemma (reveal #l (hide b) == b)
+  [SMTPat (reveal #l (hide b))]
 =
-  assert (reveal #l (hide #l b) `Seq.equal` b)
+  assert (reveal #l (hide b) `Seq.equal` b)
